SP1Chips/AddChip.lean
@@ -1,4 +1,6 @@
-import SP1Operations
+import SP1Operations.AddOperation
+import SP1Operations.RTypeReader
+import SP1Operations.CPUState
 import LeanRV32D.RiscvInstsEnd
 
 open LeanRV32D.Functions Sail
@@ -7,58 +9,18 @@ namespace AddChip
 
 section constraints
 
-def constraints
-  (Main : Vector BabyBear 23)
-  : SP1ConstraintList :=
+def constraints (Main : Vector BabyBear 23) : SP1ConstraintList :=
   let E0 : BabyBear := Main[22] - 1
-  let E2 : BabyBear := Main[22] * E0
-  let E4 : BabyBear := Main[3] + 4
-  let E6 : BabyBear := 16384 * Main[1]
-  let E8 : BabyBear := E6 + Main[2]
-  [ .assertZero E2
-  ]
-  ++ (AddOperation.constraints #v[Main[11], Main[12], Main[16], Main[17], Main[20], Main[21], Main[22]])
-  ++ (CPUState.constraints
-      { clk_high := Main[0]
-      , clk_16_24 := Main[1]
-      , clk_0_16 := Main[2]
-      , pc := Main[3] }
-      E4
-      4
-      Main[22])
-  ++ (RTypeReader.constraints
-    Main[0]
-    E8
-    -- Main[3]
-    -- 0
-    #v[Main[20], Main[21]]
-    { op_a := Main[4]
-    , op_a_memory :=
-        { prev_value := #v[Main[5], Main[6]]
-        , access_timestamp :=
-            { prev_low := Main[7]
-            , diff_low_limb := Main[8]
-            }
-        }
-    , op_a_0 := Main[9]
-    , op_b := Main[10]
-    , op_b_memory :=
-        { prev_value := #v[Main[11], Main[12]]
-        , access_timestamp :=
-            { prev_low := Main[13]
-            , diff_low_limb := Main[14]
-            }
-        }
-    , op_c := Main[15]
-    , op_c_memory :=
-        { prev_value := #v[Main[16], Main[17]]
-        , access_timestamp :=
-            { prev_low := Main[18]
-            , diff_low_limb := Main[19]
-            }
-        }
-    }
-    Main[22])
+  let E1 : BabyBear := Main[22] * E0
+  let CS0 : List SP1Constraint := AddOperation.constraints #v[Main[11], Main[12]] #v[Main[16], Main[17]] { value := #v[Main[20], Main[21]] } Main[22]
+  let E2 : BabyBear := Main[3] + 4
+  let CS1 : List SP1Constraint := CPUState.constraints { clk_0_16 := Main[2], clk_16_24 := Main[1], clk_high := Main[0], pc := Main[3] } E2 8 Main[22]
+  let E3 : BabyBear := Main[1] * 65536
+  let E4 : BabyBear := Main[2] + E3
+  let CS2 : List SP1Constraint := RTypeReader.constraints Main[0] E4 Main[3] 0 #v[Main[20], Main[21]] { op_a := Main[4], op_a_0 := Main[9], op_a_memory := { access_timestamp := { diff_low_limb := Main[8], prev_low := Main[7] }, prev_value := #v[Main[5], Main[6]] }, op_b := Main[10], op_b_memory := { access_timestamp := { diff_low_limb := Main[14], prev_low := Main[13] }, prev_value := #v[Main[11], Main[12]] }, op_c := Main[15], op_c_memory := { access_timestamp := { diff_low_limb := Main[19], prev_low := Main[18] }, prev_value := #v[Main[16], Main[17]] } } Main[22]
+  [
+    .assertZero E1
+  ] ++ CS0 ++ CS1 ++ CS2
 
 lemma bound_of_constraints (Main : Vector BabyBear 23)
     (cstrs : (constraints Main).allHold)
